\begin{equation} 
\begin{aligned}[b]
    \sum_{i=1}^n d_i^2 
    &= \sum_{i=1}^n(x_i - \bar{x})^2+(y_i - \bar{y})^2\\
    &-(u_1(x_i - \bar{x})+u_2(y_i - \bar{y}))^2 \\
    &=(1-u_1^2)\sum_{i=1}^n(x_i - \bar{x})^2+
    (1-u_2^2)\sum_{i=1}^n(y_i - \bar{y})^2\\
    &+2u_1u_2\sum_{i=1}^n(x_i - \bar{x})(y_i - \bar{y})\\
    &= (1-u_1^2)S_{xx}+
    (1-u_2^2)S_{yy}+2u_1u_2S_{xy}\\
    &=\mathbf{u}^T
    \vcenter{
        \hbox{$
        \begin{pmatrix}
        S_{xx} & S_{xy} \\
        S_{xy} & S_{yy}
        \end{pmatrix}
        $}
    } \label{eq:projection_matrix}
    \mathbf{u} = \mathbf{u}^T\mathbf{M}\mathbf{u}
\end{aligned}
\end{equation}